CFHeaps.v
@@ -3,7 +3,10 @@ Require Export LibCore LibEpsilon Shared LibMap.
 
 
 (********************************************************************)
-(* ** Representation of Heaps *)
+(* ** Heaps *)
+
+(*------------------------------------------------------------------*)
+(* ** Representation of heaps *)
 
 (** Representation of locations *)
 
@@ -19,9 +22,8 @@ Record dyn := {
 
 Definition heap := option (map loc dyn).
 
-
-(********************************************************************)
-(* ** Construction of Heaps *)
+(*------------------------------------------------------------------*)
+(* ** Construction of heaps *)
 
 (** Empty heap *)
 
@@ -47,6 +49,9 @@ Definition heap_union (h1 h2 : heap) : heap :=
 
 (********************************************************************)
 (* ** Predicate on Heaps *)
+
+(*------------------------------------------------------------------*)
+(* ** Definition of heap predicates *)
 
 (** [hprop] is the type of predicates on heaps *)
 
@@ -77,9 +82,13 @@ Definition heap_is_pack A (Hof : A -> hprop) : hprop :=
 Definition heap_is_empty_st (H:Prop) : hprop :=
   fun h => h = heap_empty /\ H.
 
+(** Star with post-conditions (predicates of type [B->hprop]) *)
 
-(********************************************************************)
-(* ** Notation for predicates *)
+Definition starpost B (Q:B->hprop) (H:hprop) : B->hprop :=
+  fun x => Q x ** H.
+
+(*------------------------------------------------------------------*)
+(* ** Notation for heap predicates *)
 
 Notation "[]" := (heap_is_empty) 
   (at level 0) : heap_scope.
@@ -104,14 +113,13 @@ Notation "l '~>' v" := (heap_is_single l (=v))
 Notation "'Hexists' x , H" := (heap_is_pack (fun x => H))
   (at level 35, x ident, H at level 200) : heap_scope.
 
+Notation "Q *** H" := (starpost Q H) (at level 40).
+
 Open Scope heap_scope.
 
 
-(********************************************************************)
-(* ** Facts *)
-
 (*------------------------------------------------------------------*)
-(* ** Properties of Star *)
+(* ** Properties of [star] *)
 
 Lemma star_neutral_l : neutral_l heap_is_star [].
 Proof. skip. Qed.
@@ -125,5 +133,145 @@ Proof. skip. Qed.
 Lemma star_assoc : LibOperation.assoc heap_is_star. 
 Proof. skip. Qed.
 
+Lemma starpost_neutral : forall B (Q:B->hprop),
+  Q *** [] = Q.
+Proof. extens. intros. unfold starpost. rewrite~ star_neutral_l. Qed.
+
+
+(*------------------------------------------------------------------*)
+(* ** Normalization of [star] *)
+
+Hint Rewrite 
+  star_neutral_l star_neutral_r star_assoc
+  starpost_neutral : rew_heap.
+
+Tactic Notation "rew_heap" :=
+  autorewrite with rew_heap.
+Tactic Notation "rew_heap" "in" "*" :=
+  autorewrite with rew_heap in *.
+Tactic Notation "rew_heap" "in" hyp(H) :=
+  autorewrite with rew_heap in H.
+
+Tactic Notation "rew_heap" "~" :=
+  rew_heap; auto_tilde.
+Tactic Notation "rew_heap" "~" "in" "*" :=
+  rew_heap in *; auto_tilde.
+Tactic Notation "rew_heap" "~" "in" hyp(H) :=
+  rew_heap in H; auto_tilde.
+
+Tactic Notation "rew_heap" "*" :=
+  rew_heap; auto_star.
+Tactic Notation "rew_heap" "*" "in" "*" :=
+  rew_heap in *; auto_star.
+Tactic Notation "rew_heap" "*" "in" hyp(H) :=
+  rew_heap in H; auto_star.
+
+
+
+(********************************************************************)
+(* ** Locality *)
+
+(*------------------------------------------------------------------*)
+(* ** Definition of [local] *)
+
+(** Type of post-conditions on values of type B *)
+
+Notation "'~~' B" := (hprop->(B->hprop)->Prop) 
+  (at level 8, only parsing) : type_scope.
+
+(** "Local" = Frame rule + consequence rule + garbage collection *)
+
+Definition local B (F:~~B) : ~~B :=
+  fun (H:hprop) (Q:B->hprop) =>
+    exists H1 H2 Q1 H',
+       H ==> H1 * H2
+    /\ F H1 Q1
+    /\ forall x, (Q1 x) * H2 ==> (Q x) * H'.
+
+(** Characterization of "local" judgments *)
+
+Definition is_local B (F:~~B) :=
+  F = local F.
+
+(** The weakening property is implied by locality *)
+
+Definition weakenable B (F:~~B) :=
+  forall H Q , F H Q ->
+  forall H' Q', H' ==> H -> Q ===> Q' -> F H' Q'.
+
+
+(*------------------------------------------------------------------*)
+(* ** Properties of [local] *)
+
+(** The [local] operator can be freely erased from a conclusion *)
+
+Lemma local_erase : forall B (F:~~B), 
+  forall H Q, F H Q -> local F H Q.
+Proof.
+  intros. exists H [] Q []. splits.
+  rew_heap~. auto. auto.
+Qed.
+
+(** Nested applications [local] are redundant *)
+
+Lemma local_local : forall B (F:~~B),
+  local (local F) = local F.
+Proof.
+  extens. intros H Q. iff M. 
+  destruct M as (H1&H2&Q1&H'&?&N&?).
+  destruct N as (H1'&H2'&Q1'&H''&?&?&?).
+  exists H1' (H2 ** H2') Q1' (H' ** H''). splits.
+  eapply pred_le_trans. eauto.
+   intros h Hh. hnf in Hh. destruct Hh as (h1&h2&?&?&?).
+   subst h. applys_to H8 H4. intuit H8. subst h1.
+   rewrite (star_comm H2). rewrite star_assoc.
+   exists __ __. splits~. exists __ __. splits~.
+  eauto.
+  intros.
+  skip. (* todo *)
+  apply~ local_erase.
+Qed.
+
+(** Elimination lemma associated with the definition of [local] *)
+
+Lemma local_elim : forall B (F:~~B) H H1 H2 H' Q1 Q,
+  is_local F -> 
+  F H1 Q1 -> 
+  H ==> H1 ** H2 -> 
+  Q1 *** H2 ===> Q *** H' ->
+  F H Q.
+Proof.
+  introv L M WH WQ. rewrite L. exists H1 H2 Q1 H'. splits.
+  auto. auto. intros. rew_heap~. apply WQ.
+Qed.
+
+(** Corrolary for the case where no garbage collection is required *)
+
+Lemma local_frame : forall B (F:~~B) H H1 H2 Q1 Q,
+  is_local F -> 
+  F H1 Q1 -> 
+  H ==> H1 ** H2 -> 
+  Q1 *** H2 ===> Q ->
+  F H Q.
+Proof.
+  intros. eapply local_elim with (H' := []); eauto. rew_heap~.
+Qed.
+
+(** Corrolary for the case where no frame is required *)
+
+Lemma local_weaken : forall B (F:~~B) H H' Q Q',
+  is_local F -> 
+  F H' Q' -> 
+  H ==> H' -> 
+  Q' ===> Q ->
+  F H Q.
+Proof.
+  intros. eapply local_frame with (H2 := []); eauto; rew_heap~.
+Qed.
+
+Lemma local_weaken' : forall B (F:~~B),
+  is_local F -> weakenable F.
+Proof. intros_all. apply* local_weaken. Qed.
+  (* todo: use only one lemma *)
 
 
